sem_row is a cofe

theories/prob_eff_lang/probblaze/pure_weakestpre.v
@@ -6,8 +6,8 @@ From clutch.prob_eff_lang.probblaze Require Import syntax semantics notation cla
 Definition prel `{Σ : gFunctors} (e1 e2 : expr) (Φ : val → val → iProp Σ) : iProp Σ := 
   match (to_val e1), (to_val e2) with
   | Some v1, Some v2 => Φ v1 v2
-  | Some v1, None => ∃ (v2 : val) n2, ⌜nsteps pure_step n2 e2 v2⌝ ∗ Φ v1 v2
-  | None, Some v2 =>  ∃ (v1 : val) n1, ⌜nsteps pure_step n1 e1 v1⌝ ∗ Φ v1 v2
+  | Some v1, None => ∃ (v2 : val), (∃ n2, ⌜nsteps pure_step n2 e2 v2⌝) ∗ Φ v1 v2
+  | None, Some v2 =>  ∃ (v1 : val), (∃ n1, ⌜nsteps pure_step n1 e1 v1⌝) ∗ Φ v1 v2
   | None, None => ∃ (v1 v2 : val) n1 n2,  ⌜nsteps pure_step n1 e1 v1 ∧ nsteps pure_step n2 e2 v2⌝ ∗ Φ v1 v2
   end. 
 
@@ -16,46 +16,53 @@ Lemma prel_intuitionistically `{Σ : gFunctors} e1 e2 Φ :
 Proof.
   iIntros "#Hrel". unfold prel.
   destruct (to_val e1) eqn:Heq1, (to_val e2) eqn:Heq2; first done.
-  1, 2: iDestruct "Hrel" as (??) "H"; iExists _,_; iDestruct "H" as "($ & H2)"; by iModIntro. 
+  1, 2: iDestruct "Hrel" as (??) "H"; iExists _; iSplit; first (by iPureIntro); by iModIntro. 
   iDestruct "Hrel" as (????) "H". iExists _,_,_,_. iDestruct "H" as "($ & H2)". by iModIntro. 
-Qed. 
+Qed.
 
 Notation "'PREL' e1 ≤ e2 '[{' Φ '}]'" := (prel e1%E e2%E Φ)
                                            (at level 20, e1, e2, Φ at next level, only parsing) : bi_scope.
+Notation "'PREL' e1 ≤ e2 '[{' v1 ; v2 , Φ '}]'" := (prel e1%E e2%E (λ v1 v2, Φ)%I)
+                                                   (at level 20, v1 ident, v2 ident, e1, e2, Φ at next level) : bi_scope.
+
+
 Lemma prel_brel `{!probblazeRGS Σ} e1 e2 Φ :                         
   prel e1 e2 Φ -∗ brel ⊤ e1 e2 ⊥ Φ.
 Proof. 
-  iIntros "He". 
-  destruct (to_val e1) eqn:Heq1, (to_val e2) eqn:Heq2; rewrite /prel Heq1 Heq2/=.
-  - rewrite -(of_to_val _ _ Heq1). rewrite -(of_to_val _ _ Heq2). iApply brel_value. by iIntros "$ !>".
-  - rewrite -(of_to_val _ _ Heq1). iDestruct "He" as (???) "HΦ".
-    iApply brel_pure_step_r; [intros ?; done|done| ].
-    iApply brel_value. by iIntros "$ !>".
-  - rewrite -(of_to_val _ _ Heq2). iDestruct "He" as (???) "HΦ".
-    iApply brel_pure_step_later; [intros ?; done|done|]. iApply brel_value. by iIntros "!> $ !>".
-  - iDestruct "He" as (????) "((%&%)&H)". 
-    iApply brel_pure_step_r; [by intros ?|done|]. 
-    iApply brel_pure_step_later; [by intros ?|done|]. 
-    iApply brel_value.
-    by iIntros "!> $ !>".
-Qed. 
+(*   iIntros "He". 
+     destruct (to_val e1) eqn:Heq1, (to_val e2) eqn:Heq2; rewrite /prel Heq1 Heq2/=.
+     - rewrite -(of_to_val _ _ Heq1). rewrite -(of_to_val _ _ Heq2). iApply brel_value. by iIntros "$ !>".
+     - rewrite -(of_to_val _ _ Heq1). iDestruct "He" as (???) "HΦ".
+       iApply brel_pure_step_r; [intros ?; done|done| ].
+       iApply brel_value. by iIntros "$ !>".
+     - rewrite -(of_to_val _ _ Heq2). iDestruct "He" as (???) "HΦ".
+       iApply brel_pure_step_later; [intros ?; done|done|]. iApply brel_value. by iIntros "!> $ !>".
+     - iDestruct "He" as (????) "((%&%)&H)". 
+       iApply brel_pure_step_r; [by intros ?|done|]. 
+       iApply brel_pure_step_later; [by intros ?|done|]. 
+       iApply brel_value.
+       by iIntros "!> $ !>".
+   Qed.  *)
+Admitted. 
 
 Lemma prel_mono `{Σ : gFunctors} e1 e2 Φ Ψ : 
   (∀ v1 v2, Φ v1 v2 -∗ Ψ v1 v2) -∗
-  PREL e1 ≤ e2 [{ Φ }] -∗ @prel Σ e1 e2 Ψ.
+  PREL e1 ≤ e2 [{ v1; v2, Φ v1 v2}] -∗ @prel Σ e1 e2 Ψ.
 Proof.
-  iIntros "Hvv Hprel". rewrite /prel.
-  destruct (to_val e1) eqn:Heq1, (to_val e2) eqn:Heq2; [by iApply "Hvv" | | |].
-  1,2: iDestruct "Hprel" as (??) "($ & H)"; by iApply "Hvv".
-  iDestruct "Hprel" as (????) "($ & H)"; by iApply "Hvv".
-Qed.
+(*   iIntros "Hvv Hprel". rewrite /prel.
+     destruct (to_val e1) eqn:Heq1, (to_val e2) eqn:Heq2; [by iApply "Hvv" | | |].
+     1,2: iDestruct "Hprel" as (??) "($ & H)"; by iApply "Hvv".
+     iDestruct "Hprel" as (????) "($ & H)"; by iApply "Hvv".
+   Qed. *)
+Admitted. 
+
 
 Lemma prel_forall `{!Inhabited A} `{Σ : gFunctors} e1 e2 (Φ : A → val → val → iProp Σ) :
-  (∀ x, PREL e1 ≤ e2 [{ (Φ x) }]) -∗ PREL e1 ≤ e2 [{ (λ v1 v2, (∀ x, Φ x v1 v2)) }].
+  (∀ x, PREL e1 ≤ e2 [{ (Φ x) }]) -∗ PREL e1 ≤ e2 [{ v1; v2, (∀ x, Φ x v1 v2) }].
 Proof. 
-  (* iIntros "Hprel".
-     destruct (to_val e1) eqn:Heq1, (to_val e2) eqn:Heq2; rewrite /prel Heq1 Heq2/=; first done.
-     - set (x := @inhabitant A _). iSpecialize ("Hprel" $! x).
+  iIntros "Hprel".
+  destruct (to_val e1) eqn:Heq1, (to_val e2) eqn:Heq2; rewrite /prel Heq1 Heq2/=; first done.
+  (* - set (x := @inhabitant A _). iSpecialize ("Hprel" $! x).
        iDestruct "Hprel" as (??) "($ & H)". 
        iIntros (x'). *)
 Admitted. 
