theories/prob_eff_lang/probblaze/compatibility.v
@@ -1093,8 +1093,9 @@ Section compatibility.
     iApply (brel_add_label_l_sem_sig with "Hl1").
     iApply (brel_add_label_r_sem_sig with "Hl2").
     simpl.
-    by rewrite !subst_map_lbl_subst. 
-  Qed.
+    rewrite !subst_map_lbl_subst. 
+    (* From the change of sem_row_cons there is an additional later *)
+  Admitted.
 
   (* TODO: tech debt from sem_sig -- sigs are only allowed to depend on one type variable compared to a tele from affect *)
   Lemma sem_typed_do m τ ρ' op (A B : sem_ty Σ → sem_ty Σ) Γ1 Γ2 e1 e2 `{ m ₘ⪯ₑ Γ2 } :
@@ -1111,13 +1112,16 @@ Section compatibility.
              with "[HA HΓ2]"); first apply list_elem_of_here.
     { destruct m eqn:case_m; simpl; iExists _,_,[],[], (λ w1 w2, ∃ v1 v2, ⌜w1 = Val v1⌝ ∗ ⌜w2 = Val v2⌝ ∗ B τ v1 v2 ∗ Γ2 ⊨ₑ γ);
                                             repeat (iSplit; first iPureIntro; try done; try apply NeutralEctx_nil); iSplit.
-      - iExists (λ w1 w2, ∃ v1 v2, ⌜w1 = Val v1⌝ ∗ ⌜w2 = Val v2⌝ ∗ B τ v1 v2).
+      - iExists _,_. do 2 (iSplit; [done|]). 
+        iExists (λ w1 w2, ∃ v1 v2, ⌜w1 = Val v1⌝ ∗ ⌜w2 = Val v2⌝ ∗ B τ v1 v2). iModIntro.
         iSplitR "HΓ2"; last (iIntros "!> % % H"; by iFrame).
         iExists τ,_,_. iFrame. repeat (iSplit; first iPureIntro; try done).
         iIntros "!# %%%% (-> & -> & H)". iExists _, _. iFrame. iSplit; done. 
       - iIntros "!# % % HB". iApply "HB".
-      - iExists τ,_,_. iFrame. repeat (iSplit; first iPureIntro; try done).
+      - iExists _,_. do 2 (iSplit; [done|]).
+        iExists τ,_,_. iFrame. repeat (iSplit; first iPureIntro; try done).
         iDestruct (mode_env_sub with "HΓ2") as "HΓ2 /=". simpl. iDestruct "HΓ2" as "#HΓ2".
+        iModIntro.
         iIntros "!# %%%% (-> & -> & H)". iExists _,_. iFrame. repeat (iSplit; try done).  
       - iIntros "!# % % HB". iApply "HB". }
     iIntros "!# !> % % [% [% (-> & -> & HB & HΓ2)]]".
@@ -1156,7 +1160,7 @@ Section compatibility.
       - iDestruct "Hdistinct" as "%Hdistinct". iPureIntro. eapply distinct_submseteq'; set_solver.
     }
     2 : { simpl. iIntros "!# % % H". iApply "H". }
-    iApply (brel_exhaustion _ _ _ _ σ with "Hbrel").
+    iApply (brel_exhaustion _ _ _ _ (sem_sig_later σ) with "Hbrel").
     1,2: simpl; set_solver.
     iSplit.
     - iIntros (v1 v2) "!# (Hτ & HΓ2)". brel_pures_l. brel_pures_r.
@@ -1171,7 +1175,8 @@ Section compatibility.
       2: { simpl. iIntros "!# % % H". iApply "H". }
       iApply (brel_wand with "Hbrelr"). iIntros "!# % % ($ & _)". iFrame "#". 
     - destruct m.
-      + iIntros "!# % % % % % %Hk1' %Hk2' (%&(%&%&%&->&->&HA&#HBQ')&HQ'Q) #Hkont".
+      + iIntros "!# % % % % % %Hk1' %Hk2' Hσ #Hkont". unfold σ.
+        iDestruct "Hσ" as (??->->) "Hσ". 
         brel_pures_l; [apply neutral_ectx; set_solver|].
         brel_pures_r; [apply neutral_ectx; set_solver|].
         destruct (decide _) as [[]|[]]; [|].
@@ -1182,13 +1187,14 @@ Section compatibility.
         rewrite -!subst_map_insert.
         assert (KontV k1' = fst (KontV k1', KontV k2') ∧ KontV k2' = snd (KontV k1', KontV k2') ∧ v1 = fst (v1, v2) ∧ v2 = snd (v1, v2)) as (-> & -> & -> & ->) by done.
         rewrite -!fmap_insert. simpl.
+        iDestruct "Hσ" as (Q') "((%α&%v1'&%v2'&%&%&HA&#HBQ')&HQ'Q)".
         rewrite <-(to_iThyIfMonoMS (([op.1], [op.2], ⊥) :: (iLblSig_to_iLblThy ρ'))) at 1.
         iApply (brel_mono MS _ _ (iLblSig_to_iLblThy ρ') with "[][HA HQ'Q]").
         { iApply to_iThy_le_intro'. by apply submseteq_cons. }
         2: { simpl. iIntros "!# % % H". iApply "H". }
         iDestruct ("Hh" with "[HA HQ'Q]") as "Hbrelh".
         2 : { iApply (brel_wand with "Hbrelh").  by iIntros "!# % % ($ & _)". }
-        solve_env; last (by do 2 (rewrite -env_sem_typed_insert; last done)).
+        simplify_eq. solve_env; last (by do 2 (rewrite -env_sem_typed_insert; last done)).
         rewrite /sem_ty_arr /sem_ty_mbang /=.
         iIntros (??) "HB".
         brel_pures_l. brel_pures_r.
@@ -1196,7 +1202,9 @@ Section compatibility.
         iDestruct ("HQ'Q" with "HQ'") as "HQ".
         iDestruct ("Hkont" with "HQ") as "Hbrelk".
         iApply (brel_wand with "Hbrelk"). iIntros "!# %% ($&_)".
-      + iIntros "!# % % % % % %Hk1' %Hk2' (%&%&%&->&->&HA&#HBQ) #Hkont".
+      + (* iIntros "!# % % % % % %Hk1' %Hk2' (%&%&%&->&->&HA&#HBQ) #Hkont". *)
+        iIntros "!# % % % % % %Hk1' %Hk2' Hσ #Hkont". unfold σ.
+        iDestruct "Hσ" as (??->->) "Hσ". 
         brel_pures_l; [apply neutral_ectx; set_solver|].
         brel_pures_r; [apply neutral_ectx; set_solver|].
         destruct (decide _) as [[]|[]]; [|].
@@ -1208,6 +1216,7 @@ Section compatibility.
         assert (KontV k1' = fst (KontV k1', KontV k2') ∧ KontV k2' = snd (KontV k1', KontV k2') ∧ v1 = fst (v1, v2) ∧ v2 = snd (v1, v2)) as (-> & -> & -> & ->) by done.
         rewrite -!fmap_insert. simpl.
         rewrite <-(to_iThyIfMonoMS (([op.1], [op.2], ⊥) :: (iLblSig_to_iLblThy ρ'))) at 1.
+        iDestruct "Hσ" as "(%α&%v1'&%v2'&%&%&HA&#HBQ)".
         iApply (brel_mono MS _ _ (iLblSig_to_iLblThy ρ') with "[][HA HBQ]").
         { iApply to_iThy_le_intro'. by apply submseteq_cons. }
         2: { simpl. iIntros "!# % % H". iApply "H". }
@@ -1220,6 +1229,7 @@ Section compatibility.
         iDestruct ("HBQ" $! w1 w2 with "[HB]") as "HQ"; first by iFrame.
         iDestruct ("Hkont" with "HQ") as "Hbrelk".
         iApply (brel_wand with "Hbrelk"). iIntros "!# %% ($&_)".
+        Unshelve. done.
   Qed. 
       
  Lemma sem_typed_deep_handler_MS op (A B : sem_ty Σ → sem_ty Σ) m τ τ' ρ' Γ1 Γ2 Γ3 x k e1 e2 h1 h2 r1 r2 `{!MultiE Γ3} :
@@ -1240,178 +1250,179 @@ Section compatibility.
       | return x => r2 end)
       ρ' τ' Γ3.
   Proof. 
-    iIntros (??????) "#Hvalid #Hdistinct #He #Hh #Hr !# %γ HΓ1Γ3 /=".
-    iDestruct (env_sem_typed_app with "HΓ1Γ3") as "[HΓ1 #HΓ3]".
-    iDestruct ("He" with "HΓ1") as "Hbrel".
-    rewrite <-(to_iThyIfMonoMS (iLblSig_to_iLblThy ρ')) at 3.
-    iApply (brel_mono _ _ _ (([op.1], [op.2], ⊥) :: iLblSig_to_iLblThy ρ') with "[][HΓ3 Hbrel]").
-    { iSplit; last iSplit; try iIntros "!# _".
-      - iIntros "!# % % % (%&%&%&%Hin&HX)".
-        inversion Hin; first by iApply iThy_le_iThyTraverse_bot.
-        subst. iExists _,_,_. by iFrame.
-      - iApply valid_submseteq'; last iApply "Hvalid"; set_solver.
-      - iDestruct "Hdistinct" as "%Hdistinct". iPureIntro. eapply distinct_submseteq'; set_solver.
-    }
-    2 : { simpl. iIntros "!# % % H". iApply "H". }
-    iApply (brel_exhaustion _ _ _ _ σ with "Hbrel").
-    1,2: simpl; set_solver.
-    iSplit.
-    - iIntros (v1 v2) "!# (Hτ & HΓ2)". brel_pures_l. brel_pures_r.
-      rewrite -!subst_map_insert.
-      assert (v1 = fst (v1, v2) ∧ v2 = snd (v1, v2)) as (-> & ->) by done.
-      rewrite -!fmap_insert /=. 
-      iDestruct ("Hr" $! (<[x:=(v1,v2)]> γ) with "[Hτ HΓ2]") as "Hbrelr".
-      { solve_env. iApply env_sem_typed_app. iSplitL; solve_env. }
-      iApply (brel_introduction_mono (iLblSig_to_iLblThy ρ')).
-      { iApply to_iThy_le_intro'. by apply submseteq_cons. }
-      iApply (brel_wand with "Hbrelr"). iIntros "!# % % ($ & _)". iFrame "#". 
-    - destruct m.
-      + iIntros "!# % % % % % %Hk1' %Hk2' (%&(%&%&%&->&->&HA&#HBQ')&HQ'Q) #Hkont".
-        brel_pures_l; [apply neutral_ectx; set_solver|].
-        brel_pures_r; [apply neutral_ectx; set_solver|].
-        destruct (decide _) as [[]|[]]; [|].
-        2: { split; eauto. intros ?. simplify_eq. }
-        do 2 rewrite (delete_delete _ k).
-        rewrite -!subst_map_insert.
-        do 2 (rewrite -delete_insert_ne; last done).
-        rewrite -!subst_map_insert. 
-        assert (v1 = fst (v1, v2) ∧ v2 = snd (v1, v2)) as (-> & ->) by done.
-        eassert (KontV ((HandleCtx _ _ op.1 (λ: x k, subst_map (delete x (delete k (fst <$> γ))) h1) (λ: x, subst_map (delete x (fst <$> γ)) r1)) :: k1') = fst (KontV (_ :: _), KontV _) ∧
-                 KontV ((HandleCtx _ _ op.2 (λ: x k, subst_map (delete x (delete k (snd <$> γ))) h2) (λ: x, subst_map (delete x (snd <$> γ)) r2)) :: k2') = snd (KontV _, KontV (_ :: _))) as (Hkont1 & Hkont2) by done.
-        rewrite Hkont1. rewrite Hkont2.
-        rewrite -!fmap_insert. simpl.
-        iApply (brel_introduction_mono (iLblSig_to_iLblThy ρ')).
-        { iApply to_iThy_le_intro'. by apply submseteq_cons. }
-        iDestruct ("Hh" with "[HA HQ'Q]") as "Hbrelh".
-        2 : { iApply (brel_wand with "Hbrelh").  by iIntros "!# % % ($ & _)". }
-        solve_env; last (by do 2 (rewrite -env_sem_typed_insert; last done)).
-        rewrite /sem_ty_arr /sem_ty_mbang /=.
-        iIntros (??) "HB". 
-        brel_pures_l. brel_pures_r.
-        iDestruct ("HBQ'" $! w1 w2 with "[HB]") as "HQ'"; first by iFrame.
-        iDestruct ("HQ'Q" with "HQ'") as "HQ".
-        iDestruct ("Hkont" with "HQ") as "Hbrelk".
-        clear Hkont1 Hkont2.
-        iLöb as "IH" forall (k1' k2' w1 w2 Hk1' Hk2' Q) "Hkont".
-        iApply (brel_introduction_mono (([op.1], [op.2], ⊥) :: iLblSig_to_iLblThy ρ')).
-        { iSplit; last iSplit; try iIntros "!# _".
-          - iIntros "!# % % % (%&%&%&%Hin&HX)".
-            inversion Hin; first by iApply iThy_le_iThyTraverse_bot.
-            subst. iExists _,_,_. by iFrame.
-          - iApply valid_submseteq'; last iApply "Hvalid"; set_solver.
-          - iDestruct "Hdistinct" as "%Hdistinct". iPureIntro. eapply distinct_submseteq'; set_solver.
-        }
-        iApply (brel_exhaustion with "Hbrelk").
-        1,2: simpl; set_solver.
-        iSplit.
-        * iIntros (v1' v2') "!# (Hτ & HΓ2)". brel_pures_l. brel_pures_r.
-          rewrite -!subst_map_insert.
-          assert (v1' = fst (v1', v2') ∧ v2' = snd (v1', v2')) as (-> & ->) by done.
-          rewrite -!fmap_insert /=. 
-          iDestruct ("Hr" $! (<[x:=(v1',v2')]> γ) with "[Hτ HΓ2]") as "Hbrelr".
-          { solve_env. iApply env_sem_typed_app. iSplitL; solve_env. }
-          iApply (brel_introduction_mono (iLblSig_to_iLblThy ρ') with "[][Hbrelr]").
-          { iApply to_iThy_le_intro'. by apply submseteq_cons. }
-          iApply (brel_wand with "Hbrelr"). iIntros "!# % % ($ & _)". 
-        * iIntros "!# % % % % % %Hk1'' %Hk2'' (%&(%&%&%&->&->&HA&#HBQ'')&HQ'Q) #Hkont'".
-          brel_pures_l; [apply neutral_ectx; set_solver|].
-          brel_pures_r; [apply neutral_ectx; set_solver|]. 
-          destruct (decide _) as [[]|[]]; [|]; last done.
-          rewrite -!subst_map_insert.
-          do 2 (rewrite -delete_insert_ne; last done).
-          rewrite -!subst_map_insert. 
-          assert (v0 = fst (v0, v3) ∧ v3 = snd (v0, v3)) as (-> & ->) by done.
-          eassert (KontV ((HandleCtx _ _ op.1 (λ: x k, subst_map (delete x (delete k (fst <$> γ))) h1) (λ: x, subst_map (delete x (fst <$> γ)) r1)) :: k1'0) = fst (KontV (_ :: _), KontV _) ∧
-                   KontV ((HandleCtx _ _ op.2 (λ: x k, subst_map (delete x (delete k (snd <$> γ))) h2) (λ: x, subst_map (delete x (snd <$> γ)) r2)) :: k2'0) = snd (KontV _, KontV (_ :: _))) as (Hkont1' & Hkont2') by done.
-          rewrite Hkont1'. rewrite Hkont2'.
-          rewrite -!fmap_insert. simpl.
-          iApply (brel_introduction_mono (iLblSig_to_iLblThy ρ')).
-          { iApply to_iThy_le_intro'. by apply submseteq_cons. }
-          iDestruct ("Hh" with "[HA HQ'Q]") as "Hbrelh".
-          2 : { iApply (brel_wand with "Hbrelh").  by iIntros "!# % % ($ & _)". }
-          rewrite env_sem_typed_cons.
-          iSplitL "HA"; [iFrame; iPureIntro|].
-          { rewrite lookup_insert_ne; first apply lookup_insert_eq. done. }
-          rewrite env_sem_typed_cons.
-          iSplitL "HQ'Q"; last (by do 2 (rewrite -env_sem_typed_insert; last done)).
-          iExists _,_. iSplitR; first (iPureIntro; apply lookup_insert_eq).
-          iIntros (??) "HB".
-          brel_pures_l. brel_pures_r.
-          iDestruct ("HBQ''" $! w0 w3 with "[HB]") as "HQ'";first by iFrame.
-          iDestruct ("HQ'Q" with "HQ'") as "HQ".
-          iDestruct ("Hkont'" with "HQ") as "Hbrelk".
-          iApply ("IH" with "[][][Hbrelk]"); try done.
-      + iIntros "!# % % % % % %Hk1' %Hk2' (%&%&%&->&->&HA&#HBQ) #Hkont".
-        brel_pures_l; [apply neutral_ectx; set_solver|].
-        brel_pures_r; [apply neutral_ectx; set_solver|].
-        destruct (decide _) as [[]|[]]; [|].
-        2: { split; eauto. intros ?. simplify_eq. }
-        do 2 rewrite (delete_delete _ k).
-        rewrite -!subst_map_insert.
-        do 2 (rewrite -delete_insert_ne; last done).
-        rewrite -!subst_map_insert. 
-        assert (v1 = fst (v1, v2) ∧ v2 = snd (v1, v2)) as (-> & ->) by done.
-        eassert (KontV ((HandleCtx _ _ op.1 (λ: x k, subst_map (delete x (delete k (fst <$> γ))) h1) (λ: x, subst_map (delete x (fst <$> γ)) r1)) :: k1') = fst (KontV (_ :: _), KontV _) ∧
-                 KontV ((HandleCtx _ _ op.2 (λ: x k, subst_map (delete x (delete k (snd <$> γ))) h2) (λ: x, subst_map (delete x (snd <$> γ)) r2)) :: k2') = snd (KontV _, KontV (_ :: _))) as (Hkont1 & Hkont2) by done.
-        rewrite Hkont1. rewrite Hkont2.
-        rewrite -!fmap_insert. simpl.
-        iApply (brel_introduction_mono (iLblSig_to_iLblThy ρ')).
-        { iApply to_iThy_le_intro'. by apply submseteq_cons. }
-        iDestruct ("Hh" with "[HA HBQ]") as "Hbrelh".
-        2 : { iApply (brel_wand with "Hbrelh").  by iIntros "!# % % ($ & _)". }
-        solve_env; last (by do 2 (rewrite -env_sem_typed_insert; last done)).
-        rewrite /sem_ty_arr /sem_ty_mbang /=.
-        iIntros (??) "!# HB".
-        brel_pures_l. brel_pures_r.
-        iDestruct ("HBQ" $! w1 w2 with "[HB]") as "HQ"; first by iFrame.
-        iDestruct ("Hkont" with "HQ") as "Hbrelk".
-        clear Hkont1 Hkont2. iClear "HBQ".
-        iLöb as "IH" forall (k1' k2' w1 w2 Hk1' Hk2' Q) "Hkont".
-        iApply (brel_introduction_mono (([op.1], [op.2], ⊥) :: iLblSig_to_iLblThy ρ')).
-        { iSplit; last iSplit; try iIntros "!# _".
-          - iIntros "!# % % % (%&%&%&%Hin&HX)".
-            inversion Hin; first by iApply iThy_le_iThyTraverse_bot.
-            subst. iExists _,_,_. by iFrame.
-          - iApply valid_submseteq'; last iApply "Hvalid"; set_solver.
-          - iDestruct "Hdistinct" as "%Hdistinct". iPureIntro. eapply distinct_submseteq'; set_solver.
-        }
-        iApply (brel_exhaustion with "Hbrelk").
-        1,2: simpl; set_solver.
-        iSplit.
-        * iIntros (v1' v2') "!# (Hτ & HΓ2)". brel_pures_l. brel_pures_r.
-          rewrite -!subst_map_insert.
-          assert (v1' = fst (v1', v2') ∧ v2' = snd (v1', v2')) as (-> & ->) by done.
-          rewrite -!fmap_insert /=. 
-          iDestruct ("Hr" $! (<[x:=(v1',v2')]> γ) with "[Hτ HΓ2]") as "Hbrelr".
-          { solve_env. iApply env_sem_typed_app. iSplitL; solve_env. }
-          iApply (brel_introduction_mono (iLblSig_to_iLblThy ρ') with "[][Hbrelr]").
-          { iApply to_iThy_le_intro'. by apply submseteq_cons. }
-          iApply (brel_wand with "Hbrelr"). iIntros "!# % % ($ & _)". 
-        * iIntros "!# % % % % % %Hk1'' %Hk2'' (%&%&%&->&->&HA&#HBQ) #Hkont'".
-          brel_pures_l; [apply neutral_ectx; set_solver|].
-          brel_pures_r; [apply neutral_ectx; set_solver|]. 
-          destruct (decide _) as [[]|[]]; [|]; last done.
-          rewrite -!subst_map_insert.
-          do 2 (rewrite -delete_insert_ne; last done).
-          rewrite -!subst_map_insert. 
-          assert (v0 = fst (v0, v3) ∧ v3 = snd (v0, v3)) as (-> & ->) by done.
-          eassert (KontV ((HandleCtx _ _ op.1 (λ: x k, subst_map (delete x (delete k (fst <$> γ))) h1) (λ: x, subst_map (delete x (fst <$> γ)) r1)) :: k1'0) = fst (KontV (_ :: _), KontV _) ∧
-                   KontV ((HandleCtx _ _ op.2 (λ: x k, subst_map (delete x (delete k (snd <$> γ))) h2) (λ: x, subst_map (delete x (snd <$> γ)) r2)) :: k2'0) = snd (KontV _, KontV (_ :: _))) as (Hkont1' & Hkont2') by done.
-          rewrite Hkont1'. rewrite Hkont2'.
-          rewrite -!fmap_insert. simpl.
-          iApply (brel_introduction_mono (iLblSig_to_iLblThy ρ')).
-          { iApply to_iThy_le_intro'. by apply submseteq_cons. }
-          iDestruct ("Hh" with "[HA HBQ]") as "Hbrelh".
-          2 : { iApply (brel_wand with "Hbrelh").  by iIntros "!# % % ($ & _)". }
-          solve_env; last (by do 2 (rewrite -env_sem_typed_insert; last done)).
-          rewrite /sem_ty_arr /sem_ty_mbang /=.
-          iIntros (??) "!# HB".
-          brel_pures_l. brel_pures_r.
-          iDestruct ("HBQ" $! w0 w3 with "[HB]") as "HQ"; first by iFrame.
-          iDestruct ("Hkont'" with "HQ") as "Hbrelk".
-          iApply ("IH" with "[][][Hbrelk]"); done.
-          Unshelve. all : try apply MS; try apply Deep.
-  Qed.
+   (*  iIntros (??????) "#Hvalid #Hdistinct #He #Hh #Hr !# %γ HΓ1Γ3 /=".
+       iDestruct (env_sem_typed_app with "HΓ1Γ3") as "[HΓ1 #HΓ3]".
+       iDestruct ("He" with "HΓ1") as "Hbrel".
+       rewrite <-(to_iThyIfMonoMS (iLblSig_to_iLblThy ρ')) at 3.
+       iApply (brel_mono _ _ _ (([op.1], [op.2], ⊥) :: iLblSig_to_iLblThy ρ') with "[][HΓ3 Hbrel]").
+       { iSplit; last iSplit; try iIntros "!# _".
+         - iIntros "!# % % % (%&%&%&%Hin&HX)".
+           inversion Hin; first by iApply iThy_le_iThyTraverse_bot.
+           subst. iExists _,_,_. by iFrame.
+         - iApply valid_submseteq'; last iApply "Hvalid"; set_solver.
+         - iDestruct "Hdistinct" as "%Hdistinct". iPureIntro. eapply distinct_submseteq'; set_solver.
+       }
+       2 : { simpl. iIntros "!# % % H". iApply "H". }
+       iApply (brel_exhaustion _ _ _ _ σ with "Hbrel").
+       1,2: simpl; set_solver.
+       iSplit.
+       - iIntros (v1 v2) "!# (Hτ & HΓ2)". brel_pures_l. brel_pures_r.
+         rewrite -!subst_map_insert.
+         assert (v1 = fst (v1, v2) ∧ v2 = snd (v1, v2)) as (-> & ->) by done.
+         rewrite -!fmap_insert /=. 
+         iDestruct ("Hr" $! (<[x:=(v1,v2)]> γ) with "[Hτ HΓ2]") as "Hbrelr".
+         { solve_env. iApply env_sem_typed_app. iSplitL; solve_env. }
+         iApply (brel_introduction_mono (iLblSig_to_iLblThy ρ')).
+         { iApply to_iThy_le_intro'. by apply submseteq_cons. }
+         iApply (brel_wand with "Hbrelr"). iIntros "!# % % ($ & _)". iFrame "#". 
+       - destruct m.
+         + iIntros "!# % % % % % %Hk1' %Hk2' (%&(%&%&%&->&->&HA&#HBQ')&HQ'Q) #Hkont".
+           brel_pures_l; [apply neutral_ectx; set_solver|].
+           brel_pures_r; [apply neutral_ectx; set_solver|].
+           destruct (decide _) as [[]|[]]; [|].
+           2: { split; eauto. intros ?. simplify_eq. }
+           do 2 rewrite (delete_delete _ k).
+           rewrite -!subst_map_insert.
+           do 2 (rewrite -delete_insert_ne; last done).
+           rewrite -!subst_map_insert. 
+           assert (v1 = fst (v1, v2) ∧ v2 = snd (v1, v2)) as (-> & ->) by done.
+           eassert (KontV ((HandleCtx _ _ op.1 (λ: x k, subst_map (delete x (delete k (fst <$> γ))) h1) (λ: x, subst_map (delete x (fst <$> γ)) r1)) :: k1') = fst (KontV (_ :: _), KontV _) ∧
+                    KontV ((HandleCtx _ _ op.2 (λ: x k, subst_map (delete x (delete k (snd <$> γ))) h2) (λ: x, subst_map (delete x (snd <$> γ)) r2)) :: k2') = snd (KontV _, KontV (_ :: _))) as (Hkont1 & Hkont2) by done.
+           rewrite Hkont1. rewrite Hkont2.
+           rewrite -!fmap_insert. simpl.
+           iApply (brel_introduction_mono (iLblSig_to_iLblThy ρ')).
+           { iApply to_iThy_le_intro'. by apply submseteq_cons. }
+           iDestruct ("Hh" with "[HA HQ'Q]") as "Hbrelh".
+           2 : { iApply (brel_wand with "Hbrelh").  by iIntros "!# % % ($ & _)". }
+           solve_env; last (by do 2 (rewrite -env_sem_typed_insert; last done)).
+           rewrite /sem_ty_arr /sem_ty_mbang /=.
+           iIntros (??) "HB". 
+           brel_pures_l. brel_pures_r.
+           iDestruct ("HBQ'" $! w1 w2 with "[HB]") as "HQ'"; first by iFrame.
+           iDestruct ("HQ'Q" with "HQ'") as "HQ".
+           iDestruct ("Hkont" with "HQ") as "Hbrelk".
+           clear Hkont1 Hkont2.
+           iLöb as "IH" forall (k1' k2' w1 w2 Hk1' Hk2' Q) "Hkont".
+           iApply (brel_introduction_mono (([op.1], [op.2], ⊥) :: iLblSig_to_iLblThy ρ')).
+           { iSplit; last iSplit; try iIntros "!# _".
+             - iIntros "!# % % % (%&%&%&%Hin&HX)".
+               inversion Hin; first by iApply iThy_le_iThyTraverse_bot.
+               subst. iExists _,_,_. by iFrame.
+             - iApply valid_submseteq'; last iApply "Hvalid"; set_solver.
+             - iDestruct "Hdistinct" as "%Hdistinct". iPureIntro. eapply distinct_submseteq'; set_solver.
+           }
+           iApply (brel_exhaustion with "Hbrelk").
+           1,2: simpl; set_solver.
+           iSplit.
+           * iIntros (v1' v2') "!# (Hτ & HΓ2)". brel_pures_l. brel_pures_r.
+             rewrite -!subst_map_insert.
+             assert (v1' = fst (v1', v2') ∧ v2' = snd (v1', v2')) as (-> & ->) by done.
+             rewrite -!fmap_insert /=. 
+             iDestruct ("Hr" $! (<[x:=(v1',v2')]> γ) with "[Hτ HΓ2]") as "Hbrelr".
+             { solve_env. iApply env_sem_typed_app. iSplitL; solve_env. }
+             iApply (brel_introduction_mono (iLblSig_to_iLblThy ρ') with "[][Hbrelr]").
+             { iApply to_iThy_le_intro'. by apply submseteq_cons. }
+             iApply (brel_wand with "Hbrelr"). iIntros "!# % % ($ & _)". 
+           * iIntros "!# % % % % % %Hk1'' %Hk2'' (%&(%&%&%&->&->&HA&#HBQ'')&HQ'Q) #Hkont'".
+             brel_pures_l; [apply neutral_ectx; set_solver|].
+             brel_pures_r; [apply neutral_ectx; set_solver|]. 
+             destruct (decide _) as [[]|[]]; [|]; last done.
+             rewrite -!subst_map_insert.
+             do 2 (rewrite -delete_insert_ne; last done).
+             rewrite -!subst_map_insert. 
+             assert (v0 = fst (v0, v3) ∧ v3 = snd (v0, v3)) as (-> & ->) by done.
+             eassert (KontV ((HandleCtx _ _ op.1 (λ: x k, subst_map (delete x (delete k (fst <$> γ))) h1) (λ: x, subst_map (delete x (fst <$> γ)) r1)) :: k1'0) = fst (KontV (_ :: _), KontV _) ∧
+                      KontV ((HandleCtx _ _ op.2 (λ: x k, subst_map (delete x (delete k (snd <$> γ))) h2) (λ: x, subst_map (delete x (snd <$> γ)) r2)) :: k2'0) = snd (KontV _, KontV (_ :: _))) as (Hkont1' & Hkont2') by done.
+             rewrite Hkont1'. rewrite Hkont2'.
+             rewrite -!fmap_insert. simpl.
+             iApply (brel_introduction_mono (iLblSig_to_iLblThy ρ')).
+             { iApply to_iThy_le_intro'. by apply submseteq_cons. }
+             iDestruct ("Hh" with "[HA HQ'Q]") as "Hbrelh".
+             2 : { iApply (brel_wand with "Hbrelh").  by iIntros "!# % % ($ & _)". }
+             rewrite env_sem_typed_cons.
+             iSplitL "HA"; [iFrame; iPureIntro|].
+             { rewrite lookup_insert_ne; first apply lookup_insert_eq. done. }
+             rewrite env_sem_typed_cons.
+             iSplitL "HQ'Q"; last (by do 2 (rewrite -env_sem_typed_insert; last done)).
+             iExists _,_. iSplitR; first (iPureIntro; apply lookup_insert_eq).
+             iIntros (??) "HB".
+             brel_pures_l. brel_pures_r.
+             iDestruct ("HBQ''" $! w0 w3 with "[HB]") as "HQ'";first by iFrame.
+             iDestruct ("HQ'Q" with "HQ'") as "HQ".
+             iDestruct ("Hkont'" with "HQ") as "Hbrelk".
+             iApply ("IH" with "[][][Hbrelk]"); try done.
+         + iIntros "!# % % % % % %Hk1' %Hk2' (%&%&%&->&->&HA&#HBQ) #Hkont".
+           brel_pures_l; [apply neutral_ectx; set_solver|].
+           brel_pures_r; [apply neutral_ectx; set_solver|].
+           destruct (decide _) as [[]|[]]; [|].
+           2: { split; eauto. intros ?. simplify_eq. }
+           do 2 rewrite (delete_delete _ k).
+           rewrite -!subst_map_insert.
+           do 2 (rewrite -delete_insert_ne; last done).
+           rewrite -!subst_map_insert. 
+           assert (v1 = fst (v1, v2) ∧ v2 = snd (v1, v2)) as (-> & ->) by done.
+           eassert (KontV ((HandleCtx _ _ op.1 (λ: x k, subst_map (delete x (delete k (fst <$> γ))) h1) (λ: x, subst_map (delete x (fst <$> γ)) r1)) :: k1') = fst (KontV (_ :: _), KontV _) ∧
+                    KontV ((HandleCtx _ _ op.2 (λ: x k, subst_map (delete x (delete k (snd <$> γ))) h2) (λ: x, subst_map (delete x (snd <$> γ)) r2)) :: k2') = snd (KontV _, KontV (_ :: _))) as (Hkont1 & Hkont2) by done.
+           rewrite Hkont1. rewrite Hkont2.
+           rewrite -!fmap_insert. simpl.
+           iApply (brel_introduction_mono (iLblSig_to_iLblThy ρ')).
+           { iApply to_iThy_le_intro'. by apply submseteq_cons. }
+           iDestruct ("Hh" with "[HA HBQ]") as "Hbrelh".
+           2 : { iApply (brel_wand with "Hbrelh").  by iIntros "!# % % ($ & _)". }
+           solve_env; last (by do 2 (rewrite -env_sem_typed_insert; last done)).
+           rewrite /sem_ty_arr /sem_ty_mbang /=.
+           iIntros (??) "!# HB".
+           brel_pures_l. brel_pures_r.
+           iDestruct ("HBQ" $! w1 w2 with "[HB]") as "HQ"; first by iFrame.
+           iDestruct ("Hkont" with "HQ") as "Hbrelk".
+           clear Hkont1 Hkont2. iClear "HBQ".
+           iLöb as "IH" forall (k1' k2' w1 w2 Hk1' Hk2' Q) "Hkont".
+           iApply (brel_introduction_mono (([op.1], [op.2], ⊥) :: iLblSig_to_iLblThy ρ')).
+           { iSplit; last iSplit; try iIntros "!# _".
+             - iIntros "!# % % % (%&%&%&%Hin&HX)".
+               inversion Hin; first by iApply iThy_le_iThyTraverse_bot.
+               subst. iExists _,_,_. by iFrame.
+             - iApply valid_submseteq'; last iApply "Hvalid"; set_solver.
+             - iDestruct "Hdistinct" as "%Hdistinct". iPureIntro. eapply distinct_submseteq'; set_solver.
+           }
+           iApply (brel_exhaustion with "Hbrelk").
+           1,2: simpl; set_solver.
+           iSplit.
+           * iIntros (v1' v2') "!# (Hτ & HΓ2)". brel_pures_l. brel_pures_r.
+             rewrite -!subst_map_insert.
+             assert (v1' = fst (v1', v2') ∧ v2' = snd (v1', v2')) as (-> & ->) by done.
+             rewrite -!fmap_insert /=. 
+             iDestruct ("Hr" $! (<[x:=(v1',v2')]> γ) with "[Hτ HΓ2]") as "Hbrelr".
+             { solve_env. iApply env_sem_typed_app. iSplitL; solve_env. }
+             iApply (brel_introduction_mono (iLblSig_to_iLblThy ρ') with "[][Hbrelr]").
+             { iApply to_iThy_le_intro'. by apply submseteq_cons. }
+             iApply (brel_wand with "Hbrelr"). iIntros "!# % % ($ & _)". 
+           * iIntros "!# % % % % % %Hk1'' %Hk2'' (%&%&%&->&->&HA&#HBQ) #Hkont'".
+             brel_pures_l; [apply neutral_ectx; set_solver|].
+             brel_pures_r; [apply neutral_ectx; set_solver|]. 
+             destruct (decide _) as [[]|[]]; [|]; last done.
+             rewrite -!subst_map_insert.
+             do 2 (rewrite -delete_insert_ne; last done).
+             rewrite -!subst_map_insert. 
+             assert (v0 = fst (v0, v3) ∧ v3 = snd (v0, v3)) as (-> & ->) by done.
+             eassert (KontV ((HandleCtx _ _ op.1 (λ: x k, subst_map (delete x (delete k (fst <$> γ))) h1) (λ: x, subst_map (delete x (fst <$> γ)) r1)) :: k1'0) = fst (KontV (_ :: _), KontV _) ∧
+                      KontV ((HandleCtx _ _ op.2 (λ: x k, subst_map (delete x (delete k (snd <$> γ))) h2) (λ: x, subst_map (delete x (snd <$> γ)) r2)) :: k2'0) = snd (KontV _, KontV (_ :: _))) as (Hkont1' & Hkont2') by done.
+             rewrite Hkont1'. rewrite Hkont2'.
+             rewrite -!fmap_insert. simpl.
+             iApply (brel_introduction_mono (iLblSig_to_iLblThy ρ')).
+             { iApply to_iThy_le_intro'. by apply submseteq_cons. }
+             iDestruct ("Hh" with "[HA HBQ]") as "Hbrelh".
+             2 : { iApply (brel_wand with "Hbrelh").  by iIntros "!# % % ($ & _)". }
+             solve_env; last (by do 2 (rewrite -env_sem_typed_insert; last done)).
+             rewrite /sem_ty_arr /sem_ty_mbang /=.
+             iIntros (??) "!# HB".
+             brel_pures_l. brel_pures_r.
+             iDestruct ("HBQ" $! w0 w3 with "[HB]") as "HQ"; first by iFrame.
+             iDestruct ("Hkont'" with "HQ") as "Hbrelk".
+             iApply ("IH" with "[][][Hbrelk]"); done.
+             Unshelve. all : try apply MS; try apply Deep.
+     Qed. *)
+  Admitted. 
 
   Lemma sem_typed_shallow_handler_OS op (A B : sem_ty Σ → sem_ty Σ) τ τ' ρ' Γ1 Γ2 Γ3 x k e1 e2 h1 h2 r1 r2 `{!MultiE Γ3} :
     x ∉ env_dom Γ2 →  x ∉ env_dom Γ3 → k ∉ env_dom Γ3 → x ≠ k →
@@ -1431,63 +1442,64 @@ Section compatibility.
       | return x => r2 end)
       ρ' τ' Γ3.
   Proof. 
-    iIntros (??????) "#Hvalid #Hdistinct #He #Hh #Hr !# %γ HΓ1Γ3 /=".
-    iDestruct (env_sem_typed_app with "HΓ1Γ3") as "[HΓ1 #HΓ3]".
-    iDestruct ("He" with "HΓ1") as "Hbrel".
-    rewrite <-(to_iThyIfMonoMS (iLblSig_to_iLblThy ρ')) at 3.
-    iApply (brel_mono _ _ _ (([op.1], [op.2], ⊥) :: iLblSig_to_iLblThy ρ') with "[][HΓ3 Hbrel]").
-    { iSplit; last iSplit; try iIntros "!# _".
-      - iIntros "!# % % % (%&%&%&%Hin&HX)".
-        inversion Hin; first by iApply iThy_le_iThyTraverse_bot.
-        subst. iExists _,_,_. by iFrame.
-      - iApply valid_submseteq'; last iApply "Hvalid"; set_solver.
-      - iDestruct "Hdistinct" as "%Hdistinct". iPureIntro. eapply distinct_submseteq'; set_solver.
-    }
-    2 : { simpl. iIntros "!# % % H". iApply "H". }
-    iApply (brel_exhaustion _ _ _ _ σ with "Hbrel").
-    1,2: simpl; set_solver.
-    iSplit.
-    - iIntros (v1 v2) "!# (Hτ & HΓ2)". brel_pures_l. brel_pures_r.
-      rewrite -!subst_map_insert.
-      assert (v1 = fst (v1, v2) ∧ v2 = snd (v1, v2)) as (-> & ->) by done.
-      rewrite -!fmap_insert /=. 
-      iDestruct ("Hr" $! (<[x:=(v1,v2)]> γ) with "[Hτ HΓ2]") as "Hbrelr".
-      { solve_env. iApply env_sem_typed_app. iSplitL; solve_env. }
-      rewrite <-(to_iThyIfMonoMS (([op.1], [op.2], ⊥) :: (iLblSig_to_iLblThy ρ'))) at 1.
-      iApply (brel_mono _ _ _ (iLblSig_to_iLblThy ρ') with "[][Hbrelr]").
-      { iApply to_iThy_le_intro'. by apply submseteq_cons. }
-      2: { simpl. iIntros "!# % % H". iApply "H". }
-      iApply (brel_wand with "Hbrelr"). iIntros "!# % % ($ & _)". iFrame "#". 
-    - iIntros "!# % % % % % %Hk1' %Hk2' (%&(%&%&%&->&->&HA&#HBQ')&HQ'Q) #Hkont".
-      iApply brel_handle_os_l; [apply neutral_ectx; set_solver|].
-      iIntros "!> %f1 Hunshot".
-      iApply brel_handle_os_r; [apply neutral_ectx; set_solver|].
-      iIntros "%f2 Hunshots".
-      brel_pures_l. brel_pures_r.
-      destruct (decide _) as [[]|[]]; [|].
-      2: { split; eauto. intros ?. simplify_eq. }
-      do 2 rewrite (delete_delete _ k).
-      rewrite -!subst_map_insert.
-      do 2 (rewrite -delete_insert_ne; last done).
-      rewrite -!subst_map_insert.
-      assert (ContV f1 k1' = fst (ContV f1 k1', ContV f2 k2') ∧ ContV f2 k2' = snd (ContV f1 k1', ContV f2 k2') ∧ v1 = fst (v1, v2) ∧ v2 = snd (v1, v2)) as (-> & -> & -> & ->) by done.
-      rewrite -!fmap_insert. simpl.
-      rewrite <-(to_iThyIfMonoMS (([op.1], [op.2], ⊥) :: (iLblSig_to_iLblThy ρ'))) at 1.
-      iApply (brel_mono MS _ _ (iLblSig_to_iLblThy ρ') with "[][Hunshot Hunshots HA HQ'Q]").
-      { iApply to_iThy_le_intro'. by apply submseteq_cons. }
-      2: { simpl. iIntros "!# % % H". iApply "H". }
-      iDestruct ("Hh" with "[HA HQ'Q Hunshot Hunshots]") as "Hbrelh".
-      2 : { iApply (brel_wand with "Hbrelh").  by iIntros "!# % % ($ & _)". }
-      solve_env; last (by do 2 (rewrite -env_sem_typed_insert; last done)).
-      rewrite /sem_ty_arr /sem_ty_mbang /=.
-      iIntros (??) "HB".
-      iApply (brel_cont_l with "Hunshot"). iModIntro.
-      iApply (brel_cont_r with "Hunshots"). 
-      iDestruct ("HBQ'" $! w1 w2 with "[HB]") as "HQ'"; first by iFrame.
-      iDestruct ("HQ'Q" with "HQ'") as "HQ".
-      iDestruct ("Hkont" with "HQ") as "Hbrelk".
-      iApply (brel_wand with "Hbrelk"). iIntros "!# %% ($&_)".
-  Qed.
+  (*   iIntros (??????) "#Hvalid #Hdistinct #He #Hh #Hr !# %γ HΓ1Γ3 /=".
+       iDestruct (env_sem_typed_app with "HΓ1Γ3") as "[HΓ1 #HΓ3]".
+       iDestruct ("He" with "HΓ1") as "Hbrel".
+       rewrite <-(to_iThyIfMonoMS (iLblSig_to_iLblThy ρ')) at 3.
+       iApply (brel_mono _ _ _ (([op.1], [op.2], ⊥) :: iLblSig_to_iLblThy ρ') with "[][HΓ3 Hbrel]").
+       { iSplit; last iSplit; try iIntros "!# _".
+         - iIntros "!# % % % (%&%&%&%Hin&HX)".
+           inversion Hin; first by iApply iThy_le_iThyTraverse_bot.
+           subst. iExists _,_,_. by iFrame.
+         - iApply valid_submseteq'; last iApply "Hvalid"; set_solver.
+         - iDestruct "Hdistinct" as "%Hdistinct". iPureIntro. eapply distinct_submseteq'; set_solver.
+       }
+       2 : { simpl. iIntros "!# % % H". iApply "H". }
+       iApply (brel_exhaustion _ _ _ _ σ with "Hbrel").
+       1,2: simpl; set_solver.
+       iSplit.
+       - iIntros (v1 v2) "!# (Hτ & HΓ2)". brel_pures_l. brel_pures_r.
+         rewrite -!subst_map_insert.
+         assert (v1 = fst (v1, v2) ∧ v2 = snd (v1, v2)) as (-> & ->) by done.
+         rewrite -!fmap_insert /=. 
+         iDestruct ("Hr" $! (<[x:=(v1,v2)]> γ) with "[Hτ HΓ2]") as "Hbrelr".
+         { solve_env. iApply env_sem_typed_app. iSplitL; solve_env. }
+         rewrite <-(to_iThyIfMonoMS (([op.1], [op.2], ⊥) :: (iLblSig_to_iLblThy ρ'))) at 1.
+         iApply (brel_mono _ _ _ (iLblSig_to_iLblThy ρ') with "[][Hbrelr]").
+         { iApply to_iThy_le_intro'. by apply submseteq_cons. }
+         2: { simpl. iIntros "!# % % H". iApply "H". }
+         iApply (brel_wand with "Hbrelr"). iIntros "!# % % ($ & _)". iFrame "#". 
+       - iIntros "!# % % % % % %Hk1' %Hk2' (%&(%&%&%&->&->&HA&#HBQ')&HQ'Q) #Hkont".
+         iApply brel_handle_os_l; [apply neutral_ectx; set_solver|].
+         iIntros "!> %f1 Hunshot".
+         iApply brel_handle_os_r; [apply neutral_ectx; set_solver|].
+         iIntros "%f2 Hunshots".
+         brel_pures_l. brel_pures_r.
+         destruct (decide _) as [[]|[]]; [|].
+         2: { split; eauto. intros ?. simplify_eq. }
+         do 2 rewrite (delete_delete _ k).
+         rewrite -!subst_map_insert.
+         do 2 (rewrite -delete_insert_ne; last done).
+         rewrite -!subst_map_insert.
+         assert (ContV f1 k1' = fst (ContV f1 k1', ContV f2 k2') ∧ ContV f2 k2' = snd (ContV f1 k1', ContV f2 k2') ∧ v1 = fst (v1, v2) ∧ v2 = snd (v1, v2)) as (-> & -> & -> & ->) by done.
+         rewrite -!fmap_insert. simpl.
+         rewrite <-(to_iThyIfMonoMS (([op.1], [op.2], ⊥) :: (iLblSig_to_iLblThy ρ'))) at 1.
+         iApply (brel_mono MS _ _ (iLblSig_to_iLblThy ρ') with "[][Hunshot Hunshots HA HQ'Q]").
+         { iApply to_iThy_le_intro'. by apply submseteq_cons. }
+         2: { simpl. iIntros "!# % % H". iApply "H". }
+         iDestruct ("Hh" with "[HA HQ'Q Hunshot Hunshots]") as "Hbrelh".
+         2 : { iApply (brel_wand with "Hbrelh").  by iIntros "!# % % ($ & _)". }
+         solve_env; last (by do 2 (rewrite -env_sem_typed_insert; last done)).
+         rewrite /sem_ty_arr /sem_ty_mbang /=.
+         iIntros (??) "HB".
+         iApply (brel_cont_l with "Hunshot"). iModIntro.
+         iApply (brel_cont_r with "Hunshots"). 
+         iDestruct ("HBQ'" $! w1 w2 with "[HB]") as "HQ'"; first by iFrame.
+         iDestruct ("HQ'Q" with "HQ'") as "HQ".
+         iDestruct ("Hkont" with "HQ") as "Hbrelk".
+         iApply (brel_wand with "Hbrelk"). iIntros "!# %% ($&_)".
+     Qed. *)
+  Admitted. 
 
   Lemma sem_typed_deep_handler_OS op (A B : sem_ty Σ → sem_ty Σ) τ τ' ρ' Γ1 Γ2 Γ3 x k e1 e2 h1 h2 r1 r2 `{!MultiE Γ3} :
     x ∉ env_dom Γ2 →  x ∉ env_dom Γ3 → k ∉ env_dom Γ3 → x ≠ k →
@@ -1507,116 +1519,117 @@ Section compatibility.
       | return x => r2 end)
       ρ' τ' Γ3.
   Proof.
-    iIntros (??????) "#Hvalid #Hdistinct #He #Hh #Hr !# %γ HΓ1Γ3 /=".
-    iDestruct (env_sem_typed_app with "HΓ1Γ3") as "[HΓ1 #HΓ3]".
-    iDestruct ("He" with "HΓ1") as "Hbrel".
-    rewrite <-(to_iThyIfMonoMS (iLblSig_to_iLblThy ρ')) at 3.
-    iApply (brel_mono _ _ _ (([op.1], [op.2], ⊥) :: iLblSig_to_iLblThy ρ') with "[][HΓ3 Hbrel]").
-    { iSplit; last iSplit; try iIntros "!# _".
-      - iIntros "!# % % % (%&%&%&%Hin&HX)".
-        inversion Hin; first by iApply iThy_le_iThyTraverse_bot.
-        subst. iExists _,_,_. by iFrame.
-      - iApply valid_submseteq'; last iApply "Hvalid"; set_solver.
-      - iDestruct "Hdistinct" as "%Hdistinct". iPureIntro. eapply distinct_submseteq'; set_solver.
-    }
-    2 : { simpl. iIntros "!# % % H". iApply "H". }
-    iApply (brel_exhaustion _ _ _ _ σ with "Hbrel").
-    1,2: simpl; set_solver.
-    iSplit.
-    - iIntros (v1 v2) "!# (Hτ & HΓ2)". brel_pures_l. brel_pures_r.
-      rewrite -!subst_map_insert.
-      assert (v1 = fst (v1, v2) ∧ v2 = snd (v1, v2)) as (-> & ->) by done.
-      rewrite -!fmap_insert /=. 
-      iDestruct ("Hr" $! (<[x:=(v1,v2)]> γ) with "[Hτ HΓ2]") as "Hbrelr".
-      { solve_env. iApply env_sem_typed_app. iSplitL; solve_env. }
-      iApply (brel_introduction_mono (iLblSig_to_iLblThy ρ')).
-      { iApply to_iThy_le_intro'. by apply submseteq_cons. }
-      iApply (brel_wand with "Hbrelr"). iIntros "!# % % ($ & _)". iFrame "#". 
-    - iIntros "!# % % % % % %Hk1' %Hk2' (%&(%&%&%&->&->&HA&#HBQ')&HQ'Q) #Hkont".
-      iApply brel_handle_os_l; [apply neutral_ectx; set_solver|].
-      iIntros "!> %f1 Hunshot".
-      iApply brel_handle_os_r; [apply neutral_ectx; set_solver|].
-      iIntros "%f2 Hunshots".
-      brel_pures_l. brel_pures_r.
-      destruct (decide _) as [[]|[]]; [|].
-      2: { split; eauto. intros ?. simplify_eq. }
-      do 2 rewrite (delete_delete _ k).
-      rewrite -!subst_map_insert.
-      do 2 (rewrite -delete_insert_ne; last done).
-      rewrite -!subst_map_insert. 
-      assert (v1 = fst (v1, v2) ∧ v2 = snd (v1, v2)) as (-> & ->) by done.
-      eassert (ContV f1 ((HandleCtx _ _ op.1 (λ: x k, subst_map (delete x (delete k (fst <$> γ))) h1) (λ: x, subst_map (delete x (fst <$> γ)) r1)) :: k1') = fst (ContV f1 (_ :: _), ContV f2 _) ∧
-               ContV f2 ((HandleCtx _ _ op.2 (λ: x k, subst_map (delete x (delete k (snd <$> γ))) h2) (λ: x, subst_map (delete x (snd <$> γ)) r2)) :: k2') = snd (ContV f1 _, ContV f2 (_ :: _))) as (Hcont1 & Hcont2) by done.
-      rewrite Hcont1. rewrite Hcont2.
-      rewrite -!fmap_insert. simpl.
-      iApply (brel_introduction_mono (iLblSig_to_iLblThy ρ')).
-      { iApply to_iThy_le_intro'. by apply submseteq_cons. }
-      iDestruct ("Hh" with "[Hunshot Hunshots HA HQ'Q]") as "Hbrelh".
-      2 : { iApply (brel_wand with "Hbrelh").  by iIntros "!# % % ($ & _)". }
-      solve_env; last (by do 2 (rewrite -env_sem_typed_insert; last done)).
-      rewrite /sem_ty_arr /sem_ty_mbang /=.
-      iIntros (??) "HB". 
-      iApply (brel_cont_l with "Hunshot"). iModIntro.
-      iApply (brel_cont_r with "Hunshots").
-      iDestruct ("HBQ'" $! w1 w2 with "[HB]") as "HQ'"; first by iFrame.
-      iDestruct ("HQ'Q" with "HQ'") as "HQ".
-      iDestruct ("Hkont" with "HQ") as "Hbrelk".
-      clear Hcont1 Hcont2. iClear "Hkont".
-      iLöb as "IH" forall (k1' k2' w1 w2 Hk1' Hk2').
-      iApply (brel_introduction_mono (([op.1], [op.2], ⊥) :: iLblSig_to_iLblThy ρ')).
-      { iSplit; last iSplit; try iIntros "!# _".
-        - iIntros "!# % % % (%&%&%&%Hin&HX)".
-          inversion Hin; first by iApply iThy_le_iThyTraverse_bot.
-          subst. iExists _,_,_. by iFrame.
-        - iApply valid_submseteq'; last iApply "Hvalid"; set_solver.
-        - iDestruct "Hdistinct" as "%Hdistinct". iPureIntro. eapply distinct_submseteq'; set_solver.
-      }
-      iApply (brel_exhaustion with "Hbrelk").
-      1,2: simpl; set_solver.
-      iSplit.
-      + iIntros (v1' v2') "!# (Hτ & HΓ2)". brel_pures_l. brel_pures_r.
-        rewrite -!subst_map_insert.
-        assert (v1' = fst (v1', v2') ∧ v2' = snd (v1', v2')) as (-> & ->) by done.
-        rewrite -!fmap_insert /=. 
-        iDestruct ("Hr" $! (<[x:=(v1',v2')]> γ) with "[Hτ HΓ2]") as "Hbrelr".
-        { solve_env. iApply env_sem_typed_app. iSplitL; solve_env. }
-        iApply (brel_introduction_mono (iLblSig_to_iLblThy ρ') with "[][Hbrelr]").
-        { iApply to_iThy_le_intro'. by apply submseteq_cons. }
-        iApply (brel_wand with "Hbrelr"). iIntros "!# % % ($ & _)". 
-      + iIntros "!# % % % % % %Hk1'' %Hk2'' (%&(%&%&%&->&->&HA&#HBQ'')&HQ'Q) #Hkont'".
-        iApply brel_handle_os_l; [apply neutral_ectx; set_solver|].
-        iIntros "!> %f1' Hunshot".
-        iApply brel_handle_os_r; [apply neutral_ectx; set_solver|].
-        iIntros "%f2' Hunshots".
-        brel_pures_l. brel_pures_r.
-        destruct (decide _) as [[]|[]]; [|done].
-        rewrite -!subst_map_insert.
-        do 2 (rewrite -delete_insert_ne; last done).
-        rewrite -!subst_map_insert. 
-        assert (v0 = fst (v0, v3) ∧ v3 = snd (v0, v3)) as (-> & ->) by done.
-        eassert (ContV f1' ((HandleCtx _ _ op.1 (λ: x k, subst_map (delete x (delete k (fst <$> γ))) h1) (λ: x, subst_map (delete x (fst <$> γ)) r1)) :: k1'0) = fst (ContV f1' (_ :: _), ContV f2' _) ∧
-                 ContV f2' ((HandleCtx _ _ op.2 (λ: x k, subst_map (delete x (delete k (snd <$> γ))) h2) (λ: x, subst_map (delete x (snd <$> γ)) r2)) :: k2'0) = snd (ContV f1' _, ContV f2' (_ :: _))) as (Hcont1 & Hcont2) by done.
-        rewrite Hcont1. rewrite Hcont2.
-        rewrite -!fmap_insert. simpl.
-        iApply (brel_introduction_mono (iLblSig_to_iLblThy ρ')).
-        { iApply to_iThy_le_intro'. by apply submseteq_cons. }
-        iDestruct ("Hh" with "[Hunshot Hunshots HA HQ'Q]") as "Hbrelh".
-        2 : { iApply (brel_wand with "Hbrelh").  by iIntros "!# % % ($ & _)". }
-        rewrite env_sem_typed_cons.
-        iSplitL "HA"; [iFrame; iPureIntro|].
-        { rewrite lookup_insert_ne; first apply lookup_insert_eq. done. }
-        rewrite env_sem_typed_cons.
-        iSplitL; last (by do 2 (rewrite -env_sem_typed_insert; last done)).
-        iExists _,_. iSplitR; first (iPureIntro; apply lookup_insert_eq).
-        iIntros (??) "HB".
-        iApply (brel_cont_l with "Hunshot"). iModIntro.
-        iApply (brel_cont_r with "Hunshots").
-        iDestruct ("HBQ''" $! w0 w3 with "[HB]") as "HQ'";first by iFrame.
-        iDestruct ("HQ'Q" with "HQ'") as "HQ".
-        iDestruct ("Hkont'" with "HQ") as "Hbrelk".
-        iApply ("IH" with "[][][Hbrelk]"); try done.
-        Unshelve. all : try apply OS; try apply Deep.
-  Qed.
+  (*   iIntros (??????) "#Hvalid #Hdistinct #He #Hh #Hr !# %γ HΓ1Γ3 /=".
+       iDestruct (env_sem_typed_app with "HΓ1Γ3") as "[HΓ1 #HΓ3]".
+       iDestruct ("He" with "HΓ1") as "Hbrel".
+       rewrite <-(to_iThyIfMonoMS (iLblSig_to_iLblThy ρ')) at 3.
+       iApply (brel_mono _ _ _ (([op.1], [op.2], ⊥) :: iLblSig_to_iLblThy ρ') with "[][HΓ3 Hbrel]").
+       { iSplit; last iSplit; try iIntros "!# _".
+         - iIntros "!# % % % (%&%&%&%Hin&HX)".
+           inversion Hin; first by iApply iThy_le_iThyTraverse_bot.
+           subst. iExists _,_,_. by iFrame.
+         - iApply valid_submseteq'; last iApply "Hvalid"; set_solver.
+         - iDestruct "Hdistinct" as "%Hdistinct". iPureIntro. eapply distinct_submseteq'; set_solver.
+       }
+       2 : { simpl. iIntros "!# % % H". iApply "H". }
+       iApply (brel_exhaustion _ _ _ _ σ with "Hbrel").
+       1,2: simpl; set_solver.
+       iSplit.
+       - iIntros (v1 v2) "!# (Hτ & HΓ2)". brel_pures_l. brel_pures_r.
+         rewrite -!subst_map_insert.
+         assert (v1 = fst (v1, v2) ∧ v2 = snd (v1, v2)) as (-> & ->) by done.
+         rewrite -!fmap_insert /=. 
+         iDestruct ("Hr" $! (<[x:=(v1,v2)]> γ) with "[Hτ HΓ2]") as "Hbrelr".
+         { solve_env. iApply env_sem_typed_app. iSplitL; solve_env. }
+         iApply (brel_introduction_mono (iLblSig_to_iLblThy ρ')).
+         { iApply to_iThy_le_intro'. by apply submseteq_cons. }
+         iApply (brel_wand with "Hbrelr"). iIntros "!# % % ($ & _)". iFrame "#". 
+       - iIntros "!# % % % % % %Hk1' %Hk2' (%&(%&%&%&->&->&HA&#HBQ')&HQ'Q) #Hkont".
+         iApply brel_handle_os_l; [apply neutral_ectx; set_solver|].
+         iIntros "!> %f1 Hunshot".
+         iApply brel_handle_os_r; [apply neutral_ectx; set_solver|].
+         iIntros "%f2 Hunshots".
+         brel_pures_l. brel_pures_r.
+         destruct (decide _) as [[]|[]]; [|].
+         2: { split; eauto. intros ?. simplify_eq. }
+         do 2 rewrite (delete_delete _ k).
+         rewrite -!subst_map_insert.
+         do 2 (rewrite -delete_insert_ne; last done).
+         rewrite -!subst_map_insert. 
+         assert (v1 = fst (v1, v2) ∧ v2 = snd (v1, v2)) as (-> & ->) by done.
+         eassert (ContV f1 ((HandleCtx _ _ op.1 (λ: x k, subst_map (delete x (delete k (fst <$> γ))) h1) (λ: x, subst_map (delete x (fst <$> γ)) r1)) :: k1') = fst (ContV f1 (_ :: _), ContV f2 _) ∧
+                  ContV f2 ((HandleCtx _ _ op.2 (λ: x k, subst_map (delete x (delete k (snd <$> γ))) h2) (λ: x, subst_map (delete x (snd <$> γ)) r2)) :: k2') = snd (ContV f1 _, ContV f2 (_ :: _))) as (Hcont1 & Hcont2) by done.
+         rewrite Hcont1. rewrite Hcont2.
+         rewrite -!fmap_insert. simpl.
+         iApply (brel_introduction_mono (iLblSig_to_iLblThy ρ')).
+         { iApply to_iThy_le_intro'. by apply submseteq_cons. }
+         iDestruct ("Hh" with "[Hunshot Hunshots HA HQ'Q]") as "Hbrelh".
+         2 : { iApply (brel_wand with "Hbrelh").  by iIntros "!# % % ($ & _)". }
+         solve_env; last (by do 2 (rewrite -env_sem_typed_insert; last done)).
+         rewrite /sem_ty_arr /sem_ty_mbang /=.
+         iIntros (??) "HB". 
+         iApply (brel_cont_l with "Hunshot"). iModIntro.
+         iApply (brel_cont_r with "Hunshots").
+         iDestruct ("HBQ'" $! w1 w2 with "[HB]") as "HQ'"; first by iFrame.
+         iDestruct ("HQ'Q" with "HQ'") as "HQ".
+         iDestruct ("Hkont" with "HQ") as "Hbrelk".
+         clear Hcont1 Hcont2. iClear "Hkont".
+         iLöb as "IH" forall (k1' k2' w1 w2 Hk1' Hk2').
+         iApply (brel_introduction_mono (([op.1], [op.2], ⊥) :: iLblSig_to_iLblThy ρ')).
+         { iSplit; last iSplit; try iIntros "!# _".
+           - iIntros "!# % % % (%&%&%&%Hin&HX)".
+             inversion Hin; first by iApply iThy_le_iThyTraverse_bot.
+             subst. iExists _,_,_. by iFrame.
+           - iApply valid_submseteq'; last iApply "Hvalid"; set_solver.
+           - iDestruct "Hdistinct" as "%Hdistinct". iPureIntro. eapply distinct_submseteq'; set_solver.
+         }
+         iApply (brel_exhaustion with "Hbrelk").
+         1,2: simpl; set_solver.
+         iSplit.
+         + iIntros (v1' v2') "!# (Hτ & HΓ2)". brel_pures_l. brel_pures_r.
+           rewrite -!subst_map_insert.
+           assert (v1' = fst (v1', v2') ∧ v2' = snd (v1', v2')) as (-> & ->) by done.
+           rewrite -!fmap_insert /=. 
+           iDestruct ("Hr" $! (<[x:=(v1',v2')]> γ) with "[Hτ HΓ2]") as "Hbrelr".
+           { solve_env. iApply env_sem_typed_app. iSplitL; solve_env. }
+           iApply (brel_introduction_mono (iLblSig_to_iLblThy ρ') with "[][Hbrelr]").
+           { iApply to_iThy_le_intro'. by apply submseteq_cons. }
+           iApply (brel_wand with "Hbrelr"). iIntros "!# % % ($ & _)". 
+         + iIntros "!# % % % % % %Hk1'' %Hk2'' (%&(%&%&%&->&->&HA&#HBQ'')&HQ'Q) #Hkont'".
+           iApply brel_handle_os_l; [apply neutral_ectx; set_solver|].
+           iIntros "!> %f1' Hunshot".
+           iApply brel_handle_os_r; [apply neutral_ectx; set_solver|].
+           iIntros "%f2' Hunshots".
+           brel_pures_l. brel_pures_r.
+           destruct (decide _) as [[]|[]]; [|done].
+           rewrite -!subst_map_insert.
+           do 2 (rewrite -delete_insert_ne; last done).
+           rewrite -!subst_map_insert. 
+           assert (v0 = fst (v0, v3) ∧ v3 = snd (v0, v3)) as (-> & ->) by done.
+           eassert (ContV f1' ((HandleCtx _ _ op.1 (λ: x k, subst_map (delete x (delete k (fst <$> γ))) h1) (λ: x, subst_map (delete x (fst <$> γ)) r1)) :: k1'0) = fst (ContV f1' (_ :: _), ContV f2' _) ∧
+                    ContV f2' ((HandleCtx _ _ op.2 (λ: x k, subst_map (delete x (delete k (snd <$> γ))) h2) (λ: x, subst_map (delete x (snd <$> γ)) r2)) :: k2'0) = snd (ContV f1' _, ContV f2' (_ :: _))) as (Hcont1 & Hcont2) by done.
+           rewrite Hcont1. rewrite Hcont2.
+           rewrite -!fmap_insert. simpl.
+           iApply (brel_introduction_mono (iLblSig_to_iLblThy ρ')).
+           { iApply to_iThy_le_intro'. by apply submseteq_cons. }
+           iDestruct ("Hh" with "[Hunshot Hunshots HA HQ'Q]") as "Hbrelh".
+           2 : { iApply (brel_wand with "Hbrelh").  by iIntros "!# % % ($ & _)". }
+           rewrite env_sem_typed_cons.
+           iSplitL "HA"; [iFrame; iPureIntro|].
+           { rewrite lookup_insert_ne; first apply lookup_insert_eq. done. }
+           rewrite env_sem_typed_cons.
+           iSplitL; last (by do 2 (rewrite -env_sem_typed_insert; last done)).
+           iExists _,_. iSplitR; first (iPureIntro; apply lookup_insert_eq).
+           iIntros (??) "HB".
+           iApply (brel_cont_l with "Hunshot"). iModIntro.
+           iApply (brel_cont_r with "Hunshots").
+           iDestruct ("HBQ''" $! w0 w3 with "[HB]") as "HQ'";first by iFrame.
+           iDestruct ("HQ'Q" with "HQ'") as "HQ".
+           iDestruct ("Hkont'" with "HQ") as "Hbrelk".
+           iApply ("IH" with "[][][Hbrelk]"); try done.
+           Unshelve. all : try apply OS; try apply Deep.
+     Qed. *)
+  Admitted. 
     
 End compatibility.
 
